src/lowparse/pulse/LowParse.Pulse.BitSum.fst
@@ -9,58 +9,6 @@ open Pulse.Lib.Slice
 #push-options "--print_universes"
 
 inline_for_extraction
-```pulse
-fn stt_cps_ifthenelse
-  (#t: Type0)
-  (y: Ghost.erased t)
-: if_combinator_weak u#4 (stt_cps u#0 #t y)
-= (cond: _)
-  (ftrue: _)
-  (ffalse: _)
-  (pre: _)
-  (t': Type0)
-  (post: _)
-  (y': _)
-{
-  if cond {
-    ftrue () pre t' post y'
-  } else {
-    ffalse () pre t' post y'
-  }
-}
-```
-
-inline_for_extraction
-let validate_bitsum'
-  (#t: eqtype)
-  (#tot: pos)
-  (#cl: uint_t tot t)
-  (#b: bitsum' cl tot)
-  (f: filter_bitsum'_t b)
-  (d: destr_bitsum'_t b)
-  (#k: parser_kind)
-  (#p: parser k t)
-  (w: validate_and_read p)
-: Pure (validate_and_read (tot_parse_bitsum' b p))
-    (requires (k.parser_kind_subkind == Some ParserStrong))
-    (ensures (fun _ -> True))
-= [@@inline_let]
-  let _ = synth_bitsum'_injective b in
-    (validate_and_read_synth
-      (validate_and_read_filter
-        w
-        (filter_bitsum' b)
-        (fun x -> f x)
-      )
-      (synth_bitsum' b)
-      (d
-        stt_cps
-        stt_cps_ifthenelse
-        (fun k pre t' post phi -> phi k)
-      )
-    )
-
-inline_for_extraction
 let jump_bitsum' 
   (#t: eqtype)
   (#tot: pos)
